atomic_pcas.v
@@ -33,7 +33,8 @@ Section atomic_pair.
 
   Local Opaque β.
   
-  Lemma pcas_seq_spec: seq_spec N pcas_seq ϕ α β ⊤.
+  (* TODO: This needs updating for the new atomic_syncer.
+  Lemma pcas_seq_spec x: atomic_seq_spec ϕ α β ⊤ pcas_seq x.
   Proof.
     iIntros (_ l) "!# _". wp_seq. iPureIntro.
     iIntros (x Φ g HN) "(#Hh & Hg & #Hα & HΦ)".
@@ -75,6 +76,6 @@ Section atomic_pair.
     iDestruct (atomic_spec with "[Hl1 Hl2]") as "Hspec"=>//.
     - apply pcas_seq_spec.
     - iFrame "Hh". iExists l1, l2, x1, x2. iFrame. eauto.
-  Qed.
+  Qed.*)
 End atomic_pair.
 
